src/tree/layer3/OrderedMapImpl.dfy
@@ -1,717 +1,33 @@
-include "../../../src/tree/BinTreeIntClara.dfy"
+include "../../../src/tree/Tree.dfy"
+include "../../../src/tree/SearchTree.dfy"
 include "../../../src/tree/layer1/OrderedMap.dfy"
 
-
-class OrderedMapIteratorImpl extends OrderedMapIterator{
-
-ghost var parent:OrderedMapImpl;
-  ghost var stackSK: seq<tree<TNode>>;//esto debería ser una Stack
-  var stack:seq<TNode>;
-  var index:int;  
-
-  constructor(p:OrderedMapImpl)
-  requires p.Valid()
-  ensures Valid() 
-  ensures Parent()==p
-  ensures Traversed()=={}
-  { parent:=p;
-    new;
-    stackSK:=[];
-    stack := [];
-    index:=0;
-    if (p.tree.root!=null)
-    { descendAndPush(p.tree.root,p.tree.skeleton,null,Empty);
-      assert index==|traversed()|==0;
-      traversedRelation();
-    }
-
-  }
-
-
-
-method {:verify false} descendAndPush(n:TNode,ghost sk: tree<TNode>, p:TNode?, ghost pk:tree<TNode>)
-modifies this
-requires Parent().Valid()
-requires ValidStack() 
-requires Tree.ValidRec(n,sk) 
-requires Tree.SearchTreeRec(sk)
-requires  n in Parent().Repr()
-requires elems(sk) <= Parent().Repr()
-requires (forall i | 0 <= i < |stackSK| :: elems(sk) < elems(stackSK[i])) 
-
-requires stack !=[] ==> Tree.LeftPathAux(n,parent.tree.skeleton)==[n]+Tree.LeftPathAux(stack[0],parent.tree.skeleton)
-requires stack == [] ==> [n] == Tree.LeftPathAux(n, parent.tree.skeleton) 
-requires stack != [] ==> stack==Tree.LeftPathAux(stack[0],parent.tree.skeleton)
-
-requires p!=null ==> p in Parent().Repr() && Tree.ValidRec(p,pk) && Tree.SearchTreeRec(pk) && p.right==n && pk.right==sk
-requires p==null ==> index==0 && stack==[] && sk==parent.tree.skeleton
-requires p != null ==> index==|set m | m in elems(parent.tree.skeleton) && m.key < p.key|
-
-ensures Parent().Valid() 
-ensures Parent()==old(Parent()) && Parent().Repr()==old(Parent().Repr())
-ensures ValidStack()
-ensures stack!=[] && stack == Tree.LeftPathAux(stack[0],parent.tree.skeleton)
-ensures p==null ==> index==0
-ensures p!=null ==> index==old(index)+1
-ensures p!=null ==> (set m | m in elems(parent.tree.skeleton) && m.key < stack[0].key)==(set m | m in elems(parent.tree.skeleton) && m.key < p.key)+{p} 
-ensures p==null ==> (set m | m in elems(parent.tree.skeleton) && m.key < stack[0].key)=={} 
-//ensures index==|(set m | m in elems(parent.tree.skeleton) && m.key < stack[0].key)|
-
-
-{
- var current:TNode? := n; var currentSK:tree<TNode>:=sk;
- ghost var oset;
- if (p!=null) {oset:=set m | m in elems(parent.tree.skeleton) && m.key < p.key;}
- else {oset:={};}
-
-assert n==current;
-assert current!=null;
-assert stack!=[] ==> Tree.LeftPathAux(n,parent.tree.skeleton)==[n]+Tree.LeftPathAux(stack[0],parent.tree.skeleton);
-assert stack==[] ==> [current] == Tree.LeftPathAux(current, parent.tree.skeleton);
-
-//assert p!=null && current!=null ==> 
-//  (set m | m in elems(parent.tree.skeleton) && m.key <= current.key) == (set m | m in elems(parent.tree.skeleton) && m.key <= p.key) + (set m | m in elems(sk) && m.key <= current.key);
-//assert p==null ==>  traversed()== (set m | m in elems(sk) && m.key <= current.key);
-//assert current==null ==> traversed() == (set m | m in elems(parent.tree.skeleton) && m.key <= p.key);
-
-
-
- while (current != null)
-  decreases currentSK
-  invariant Parent().Valid() && Parent().Repr()==old(Parent().Repr())
-  invariant elems(currentSK) <= Parent().Repr()
-  invariant Tree.ValidRec(current,currentSK)
-  invariant Tree.SearchTreeRec(currentSK)
-  invariant (forall i | 0 <= i < |stackSK| :: elems(currentSK) < elems(stackSK[i])) 
-  invariant ValidStack()
-  invariant current!=null || stack != []
-  invariant (current!=null && stack!=[]) ==>  Tree.LeftPathAux(current,parent.tree.skeleton)==[current]+Tree.LeftPathAux(stack[0],parent.tree.skeleton)
-  invariant stack!=[] ==> stack == Tree.LeftPathAux(stack[0],parent.tree.skeleton)
-  invariant stack==[] && current != null ==> [current]==Tree.LeftPathAux(current, parent.tree.skeleton)
-  invariant index==old(index)
-  invariant p!=null ==> p in Parent().Repr() && Tree.ValidRec(p,pk) && Tree.SearchTreeRec(pk) && p.right==n && pk.right==sk
-  invariant p!=null ==> oset == set m | m in elems(parent.tree.skeleton) && m.key < p.key
-  invariant p==null ==> oset == {}
-  invariant p==null && stack!=[] ==> stack[0].left==current
-  invariant p==null && stack!=[] ==> 
-    (set m | m in elems(parent.tree.skeleton) && m.key < stack[0].key)==
-    (set m | m in elems(currentSK) && m.key < stack[0].key)
-  /*invariant p==null && stack!=[] ==> 
-    (set m | m in elems(sk) && m.key < stack[0].key)==
-    (set m | m in elems(currentSK) && m.key < stack[0].key)*/
-
-  /*invariant p==null && current!=null ==>  
-    (set m | m in elems(parent.tree.skeleton) && m.key < current.key) ==
-    (set m | m in elems(currentSK) && m.key < current.key)*/
-
-  /*invariant p!=null && stack!=[] ==>
-    (set m | m in elems(parent.tree.skeleton) && m.key < stack[0].key)==
-    ((set m | m in elems(parent.tree.skeleton) && m.key < p.key) + {p} +
-    (set m | m in elems(currentSK) && m.key < stack[0].key))*/
- 
-
-  //invariant current != n  ==> traversed() == (set m | m in elems(parent.tree.skeleton) && m.key <= p.key)+(if (current!=null) then (set m | m in elems(sk) && m.key < current.key) else {})
-  //invariant p!=null && current!=null ==> traversed()== (set m | m in elems(parent.tree.skeleton) && m.key <= p.key) + (set m | m in elems(sk) && m.key <= current.key)
-  //invariant current==null ==> traversed() == (set m | m in elems(parent.tree.skeleton) && m.key <= p.key)
- {
-
-   var ostack:=stack;
-   var ostackSK:= stackSK;
-   var ocurrent:=current;   
-   var ocurrentSK:=currentSK;
-   var oindex:=index;
-
-   assert (current !=null && stack!=[]) ==> Tree.LeftPathAux(current,parent.tree.skeleton)==[current]+Tree.LeftPathAux(ostack[0],parent.tree.skeleton);
-      
-  
-   stack:=[current]+stack;
-   stackSK:=[currentSK]+stackSK;
-   
-      assert stackSK[1..|stackSK|]==ostackSK[0..|ostackSK|];
-      assert stack[1..|stack|]==ostack[0..|ostack|];
-      assert stack[0]==current;
-      assert stackSK[0]==currentSK;
-      assert current!=null && stack!=[];
-    
-      assert current.left!=null ==> Tree.LeftPathAux(current.left,parent.tree.skeleton)==[current.left]+Tree.LeftPathAux(stack[0],parent.tree.skeleton)
-      by{
-         assert stack != [];
-         Tree.propLeftPath(current,currentSK,parent.tree.root,parent.tree.skeleton);
-        } 
-
-   current:=current.left;
-   currentSK:=currentSK.left;
-     assert stack!=[];
-     assert current!=null ==> Tree.LeftPathAux(current,parent.tree.skeleton)==[current]+Tree.LeftPathAux(stack[0],parent.tree.skeleton);
-     assert stack==[] && current != null ==> [current]==Tree.LeftPathAux(current, parent.tree.skeleton);
-     
-     if (ostack==[]) {
-       assert stack==[ocurrent]==Tree.LeftPathAux(ocurrent,parent.tree.skeleton);
-       }
-     else{
-       calc =={
-         stack;
-         [stack[0]]+stack[1..|stack|];
-         [stack[0]]+ostack[0..|ostack|];
-         {assert ostack[0..|ostack|]==Tree.LeftPathAux(ostack[0],parent.tree.skeleton);}
-         [stack[0]]+Tree.LeftPathAux(ostack[0],parent.tree.skeleton);
-         {assert stack[1]==ostack[0];}
-         [stack[0]]+Tree.LeftPathAux(stack[1],parent.tree.skeleton);
-         {assert Tree.LeftPathAux(stack[0],parent.tree.skeleton)==[stack[0]]+Tree.LeftPathAux(stack[1],parent.tree.skeleton);}
-         Tree.LeftPathAux(stack[0],parent.tree.skeleton);
-        }   
-      } 
-
-  assert ValidStack();
-  
-
-  if (p==null)
-  { assert (set m | m in elems(parent.tree.skeleton) && m.key < stack[0].key)==
-  (set m | m in elems(parent.tree.skeleton) && m.key < ocurrent.key);
-  assume (set m | m in elems(parent.tree.skeleton) && m.key < ocurrent.key)==
-      (set m | m in elems(ocurrentSK.left) && m.key < ocurrent.key);
-  assert (set m | m in elems(ocurrentSK.left) && m.key < ocurrent.key)==
-  (set m | m in elems(currentSK) && m.key < stack[0].key);
-  }
-  else{
-   assume (set m | m in elems(parent.tree.skeleton) && m.key < stack[0].key)==
-    ((set m | m in elems(parent.tree.skeleton) && m.key < p.key) + {p} +
-    (set m | m in elems(currentSK) && m.key < stack[0].key));
-  }
- }
-   assert current==null && stack!=[] && stack == Tree.LeftPathAux(stack[0],parent.tree.skeleton);
-   assert currentSK==Empty;
-  
-  
-  if (p==null)
-    { assert (set m | m in elems(parent.tree.skeleton) && m.key < stack[0].key)=={};
-      assert index == 0 == |traversed()|;
-    }
-  else
-  //if (p!=null)
-  { assert old(index)== |(set m | m in elems(parent.tree.skeleton) && m.key < p.key)|;
- 
-    assume
-    (set m | m in elems(parent.tree.skeleton) && m.key < stack[0].key)==
-    (set m | m in elems(parent.tree.skeleton) && m.key < p.key) + {p} +
-    (set m | m in elems(currentSK) && m.key < stack[0].key);
-   assert  
-    (set m | m in elems(parent.tree.skeleton) && m.key < stack[0].key)==
-    (set m | m in elems(parent.tree.skeleton) && m.key < p.key) + {p};
-   calc{
-       |traversed()|;
-       |(set m | m in elems(parent.tree.skeleton) && m.key < stack[0].key)|;
-       |(set m | m in elems(parent.tree.skeleton) && m.key < p.key) + {p}|;
-       {assert p !in (set m | m in elems(parent.tree.skeleton) && m.key < p.key);}
-       |(set m | m in elems(parent.tree.skeleton) && m.key < p.key)| + 1;
-       old(index)+1;
-       index+1;
-    } 
-     index:=index+1;
-  } 
-
-     
-
- 
-
-
-
-}
-
-
-/*method {:verify false} descendAndPush(n:TNode,ghost sk: tree<TNode>)
-modifies this
-requires Parent().Valid()
-requires ValidStack() 
-requires Tree.ValidRec(n,sk) 
-requires Tree.SearchTreeRec(sk)
-requires  n in Parent().Repr()
-requires elems(sk) <= Parent().Repr()
-requires (forall i | 0 <= i < |stackSK| :: elems(sk) < elems(stackSK[i])) 
-
-requires stack !=[] ==> Tree.LeftPathAux(n,parent.tree.skeleton)==[n]+Tree.LeftPathAux(stack[0],parent.tree.skeleton)
-requires stack == [] ==> [n] == Tree.LeftPathAux(n, parent.tree.skeleton) 
-requires stack!=[] ==> stack==Tree.LeftPathAux(stack[0],parent.tree.skeleton)
-
-
-ensures Parent().Valid() && Parent().Repr()==old(Parent().Repr())
-ensures ValidStack()
-ensures stack!=[] && stack == Tree.LeftPathAux(stack[0],parent.tree.skeleton)
-{
- var current:TNode? := n; var currentSK:tree<TNode>:=sk;
-assert n==current;
-assert current!=null;
-assert stack!=[] ==> Tree.LeftPathAux(n,parent.tree.skeleton)==[n]+Tree.LeftPathAux(stack[0],parent.tree.skeleton);
-assert stack==[] ==> [current] == Tree.LeftPathAux(current, parent.tree.skeleton);
-
- while (current != null)
-  decreases currentSK
-  invariant Parent().Valid() && Parent().Repr()==old(Parent().Repr())
-  invariant elems(currentSK) <= Parent().Repr()
-  invariant Tree.ValidRec(current,currentSK)
-  invariant Tree.SearchTreeRec(currentSK)
-  invariant (forall i | 0 <= i < |stackSK| :: elems(currentSK) < elems(stackSK[i])) 
-  invariant ValidStack()
-  invariant current!=null || stack != []
-  invariant (current!=null && stack!=[]) ==> Tree.LeftPathAux(current,parent.tree.skeleton)==[current]+Tree.LeftPathAux(stack[0],parent.tree.skeleton)
-  invariant stack!=[] ==> stack == Tree.LeftPathAux(stack[0],parent.tree.skeleton)
-  invariant stack==[] && current != null ==> [current]==Tree.LeftPathAux(current, parent.tree.skeleton)
- {
-
-   var ostack:=stack;
-   var ostackSK:= stackSK;
-   var ocurrent:=current;
-   assert (current !=null && stack!=[]) ==> Tree.LeftPathAux(current,parent.tree.skeleton)==[current]+Tree.LeftPathAux(ostack[0],parent.tree.skeleton);
-      
-   stack:=[current]+stack;
-   stackSK:=[currentSK]+stackSK;
-   
-      assert stackSK[1..|stackSK|]==ostackSK[0..|ostackSK|];
-      assert stack[1..|stack|]==ostack[0..|ostack|];
-      assert stack[0]==current;
-      assert stackSK[0]==currentSK;
-      assert current!=null && stack!=[];
-    
-      assert current.left!=null ==> Tree.LeftPathAux(current.left,parent.tree.skeleton)==[current.left]+Tree.LeftPathAux(stack[0],parent.tree.skeleton)
-      by{
-         assert stack != [];
-         Tree.propLeftPath(current,currentSK,parent.tree.root,parent.tree.skeleton);
-        }
-    
-
-   current:=current.left;
-   currentSK:=currentSK.left;
-     assert stack!=[];
-     assert current!=null ==> Tree.LeftPathAux(current,parent.tree.skeleton)==[current]+Tree.LeftPathAux(stack[0],parent.tree.skeleton);
-     assert stack==[] && current != null ==> [current]==Tree.LeftPathAux(current, parent.tree.skeleton);
-     
-     if (ostack==[]) {
-       assert stack==[ocurrent]==Tree.LeftPathAux(ocurrent,parent.tree.skeleton);
-       }
-     else{
-       calc =={
-         stack;
-         [stack[0]]+stack[1..|stack|];
-         [stack[0]]+ostack[0..|ostack|];
-         {assert ostack[0..|ostack|]==Tree.LeftPathAux(ostack[0],parent.tree.skeleton);}
-         [stack[0]]+Tree.LeftPathAux(ostack[0],parent.tree.skeleton);
-         {assert stack[1]==ostack[0];}
-         [stack[0]]+Tree.LeftPathAux(stack[1],parent.tree.skeleton);
-         {assert Tree.LeftPathAux(stack[0],parent.tree.skeleton)==[stack[0]]+Tree.LeftPathAux(stack[1],parent.tree.skeleton);}
-         Tree.LeftPathAux(stack[0],parent.tree.skeleton);
-        }   
-  } 
-
-  assert ValidStack();
- }
-
-   assert current==null && stack!=[] && stack == Tree.LeftPathAux(stack[0],parent.tree.skeleton);
-
-
-}*/
-
-
-
-/*lemma {:verify false} absurdo(sk:tree<TNode>)
- requires |stack|==|stackSK|>0
- requires parent.Valid() 
- requires forall i | 0<=i<|stack| :: stack[i] in Parent().Repr()
- requires forall i | 0<=i<|stackSK| ::elems(stackSK[i]) <= Parent().Repr()
- requires forall i | 0<=i<|stackSK| :: Tree.ValidRec(stack[i],stackSK[i])
-requires (forall i | 1 <= i < |stackSK| :: elems(sk) !! reachableFromStack(i))
-requires elems(sk)!!reachableFromStack(0)
-ensures (forall i | 0 <= i < |stackSK| :: elems(sk) !! reachableFromStack(i))
-{
-  forall i | 0 <= i < |stackSK| ensures elems(sk) !! reachableFromStack(i)
-  {
-    if (i==0){ assert elems(sk)!!reachableFromStack(0);}
-    else { assert elems(sk) !! reachableFromStack(i);}
-  }
-
-}*/
-
-
-function Parent(): UnorderedMap
-    reads this
-    ensures Parent() is OrderedMapImpl
-{ parent }
-
-
-
-
-
-
-static function reachableFrom(n:TNode,sk:tree<TNode>):set<TNode>  
-reads elems(sk)
-requires Tree.ValidRec(n,sk)
-requires Tree.SearchTreeRec(sk)
-ensures forall m | m in reachableFrom(n,sk) :: m.key >= n.key 
-{ Tree.elemsProps(n,sk);
-  {n}+elems(sk.right)
-}
-
-function reachableFromStack(i:int):set<TNode>
- reads this,Parent(), Parent().Repr()
- requires 0 <= i < |stack|==|stackSK|
- requires parent.Valid() 
- requires stack[i] in Parent().Repr()
- requires elems(stackSK[i]) <= Parent().Repr()
- requires Tree.ValidRec(stack[i],stackSK[i])
- requires Tree.SearchTreeRec(stackSK[i])
- ensures reachableFromStack(i) <= Parent().Repr()
- ensures forall m | m in reachableFromStack(i) :: m.key >= stack[i].key
-{ reachableFrom(stack[i],stackSK[i])}
-//{ {stack[i]} + elems(stackSK[i].right)}
-
-function reachableFromStacks():set<TNode>
- reads this,Parent(), Parent().Repr()
-  requires parent.Valid() && ValidStack()
- ensures stack==[] ==> reachableFromStacks()=={}
-  ensures reachableFromStacks() <= Parent().Repr()
-
-{   assert unions<TNode>(set i | 0 <= i < |stack| :: reachableFromStack(i)) <= elems(parent.tree.skeleton)
-    by {
-     assert forall s | s in (set i | 0 <= i < |stack| :: reachableFromStack(i)) :: s <= Parent().Repr();
-      unionsContained<TNode>(set i | 0 <= i < |stack| :: reachableFromStack(i),elems(parent.tree.skeleton));
-      assert elems(parent.tree.skeleton) <= Parent().Repr();
-      }
-      
-  unions<TNode>(set i | 0 <= i < |stack| :: reachableFromStack(i))
-  
-}
-
- lemma reachableFromStackProps(i:int)
-  requires parent.Valid() && ValidStack()
-  requires stack!=[] && stack == Tree.LeftPathAux(stack[0],parent.tree.skeleton)
-  requires 0 <= i < |stack|
-  ensures forall m | m in reachableFromStack(i) :: m.key >= stack[i].key
-  ensures  reachableFromStack(i) !! traversed()
-  ensures forall n,m | n in traversed() && m in reachableFromStack(i):: n.key < m.key
-
-
- lemma reachableFromStacksProps(i:int,j:int)
-  requires parent.Valid() && ValidStack()
-  requires stack!=[] && stack == Tree.LeftPathAux(stack[0],parent.tree.skeleton)
-  requires 0 <= i < j < |stack|
-  ensures  reachableFromStack(i) !! reachableFromStack(j)
-  ensures forall n,m | n in  reachableFromStack(i) && m in reachableFromStack(j):: n.key < m.key
-
-  lemma reachableFromStacksPropsI(n:TNode)
-  requires parent.Valid() && ValidStack()
-  requires stack!=[] && stack == Tree.LeftPathAux(stack[0],parent.tree.skeleton)
-  requires n in reachableFromStacks()
-  ensures exists i | 0 <= i < |stack| :: n in reachableFromStack(i)
-
-lemma skeletonReachableFromStacksProp(n:TNode)
-  requires parent.Valid() && ValidStack()
-  requires stack!=[] && stack == Tree.LeftPathAux(stack[0],parent.tree.skeleton)
-  requires n in elems(parent.tree.skeleton) && n.key >= stack[0].key
-  ensures exists i | 0 <= i < |stack| :: n in reachableFromStack(i) 
-  ensures n in reachableFromStacks()
-
-function unions<A> (ss:set<set<A>>):set<A>
-  {
-    if (ss=={}) then {}
-    else 
-     var s:| s in ss;
-     s+unions(ss-{s})
-  }
-lemma unionsContained<A>(ss:set<set<A>>,u:set<A>)
-requires forall s | s in ss :: s <= u
-ensures unions(ss) <= u
-{}
-
-
-
-predicate ValidStack()
-    reads this, Parent(), Parent().Repr()
-    requires parent.Valid()
- { 
-   |stack|==|stackSK| &&  
-    (forall i | 0 <= i < |stack| :: stack[i] in Parent().Repr()) &&
-    (forall i | 0 <= i < |stackSK| :: elems(stackSK[i]) <= Parent().Repr()) && 
-    (forall i,j | 0 <= i < j < |stackSK| :: elems(stackSK[i]) < elems(stackSK[j])) && //puede que se deduzca de leftPathAux
-    (forall i | 0 <= i < |stack| :: Tree.ValidRec(stack[i],stackSK[i])) &&
-    (forall i | 0 <= i < |stackSK| :: Tree.SearchTreeRec(stackSK[i])) //&&
-    //stack!=[] ==> stack[0] in elems(parent.tree.skeleton) && stack == Tree.LeftPathAux(stack[0],parent.tree.skeleton)
-   // (forall i,j | 0 <= i < j < |stack| :: reachableFromStack(i)!!reachableFromStack(j)) && 
-   // (forall i | 0 <= i < |stack| :: reachableFromStack(i)!!traversed()) && 
-   // (forall i, n, m | 0 <= i < |stack| && n in traversed() && m in reachableFromStack(i):: n.key < m.key) && 
-   // (forall i,j,n,m | 0 <= i < j < |stack| && n in reachableFromStack(i) && m in reachableFromStack(j):: n.key < m.key)&&
-   // (stack !=[] ==> |stack| == |Tree.LeftPathAux(stack[0],parent.tree.skeleton)|) && 
-   // (forall i | 0 <= i < |stack|  :: stack[i]==Tree.LeftPathAux(stack[0],parent.tree.skeleton)[i])
- }
-
-lemma elemsStack()
-requires Parent().Valid() && ValidStack()
-requires parent.Valid() && |stack|==|stackSK|
-requires stack!=[] && stack == Tree.LeftPathAux(stack[0],parent.tree.skeleton)
-ensures elems(parent.tree.skeleton)==traversed()+ reachableFromStacks()
-{ 
- 
- forall n | n in elems(parent.tree.skeleton)
- ensures n in traversed() || n in reachableFromStacks()
- {
-   if (n.key < stack[0].key) {assert n in traversed();}
-   else{
-      skeletonReachableFromStacksProp(n);
-      }
- }
- 
- assert traversed() <= elems(parent.tree.skeleton);
- assert reachableFromStacks() <= elems(parent.tree.skeleton);
- assert elems(parent.tree.skeleton)>=traversed()+ reachableFromStacks();
- }
-
-predicate Valid()
-    reads this, Parent(), Parent().Repr()
-
-{   Parent().Valid() &&
-    ValidStack() &&
-    (stack!=[] ==> stack == Tree.LeftPathAux(stack[0],parent.tree.skeleton)) && 
-    //elems(parent.tree.skeleton)==traversed()+ reachableFromStacks() &&
-    index==|traversed()| 
-
-}
-
-//Node es descendiente de los que hay en la pila: usar leftPathAux
-//elems(skeleton) ==traversed()+ reachableFromStacks()+elems(stack[0].left)
-function traversed():set<TNode>
-      reads this,Parent(), Parent().Repr()
-      requires parent.Valid()
-      requires stack!=[] ==> stack[0] in Parent().Repr()
-  { if (stack==[]) then elems(parent.tree.skeleton) 
-    else 
-      (set n | n in elems(parent.tree.skeleton) && n.key < stack[0].key :: n)
-  }
-
-
-
-function Traversed():set<K>
-    reads this, Parent(), Parent().Repr()
-    requires Parent().Valid() 
-    requires Valid()
-    ensures Traversed() <= (Parent().Model().Keys)
-    ensures forall x,y | x in Traversed() && y in Parent().Model().Keys-Traversed() :: x < y
-{   
- if (stack==[]) then Parent().Model().Keys
-  else 
-   (set m | m in Parent().Model().Keys && m < stack[0].key)
-  
-}
-
-lemma {:verify false} traversedRelation()
-requires Valid()
-ensures Traversed()==(set n | n in traversed():: n.key)
-ensures |Traversed()|==|traversed()|
-{ 
-  if (stack==[]) {
-    parent.tree.ModelRelationWithSkeletonAllKeys();
-
-  }
-  else {parent.tree.ModelRelationWithSkeletonKeys(stack[0].key);}
-
-  assert Traversed()==(set n | n in traversed():: n.key);
-  sizes(Traversed(),(set n | n in traversed():: n.key));
-  assert |Traversed()|==|(set n | n in traversed():: n.key)|;
-  assert |(set n | n in traversed():: n.key)| == |traversed()|;
-  
-}
-
-
-
-
-function method {:verify true} Peek():pairKV 
-    reads this, Parent(), Parent().Repr()
-    requires Valid()
-    requires Parent().Valid()
-    requires HasNext()
-    ensures Peek() in Parent().Model().Items &&
-            key(Peek()) !in Traversed() 
-    ensures key(Peek())==elemth(Parent().Model().Keys,|Traversed()|)  
-    ensures value(Peek()) == Parent().Model()[key(Peek())]      
-    ensures forall k | k in Traversed() :: k < key(Peek())
-    ensures forall k | k in Parent().Model().Keys-Traversed()-{key(Peek())} :: key(Peek()) < k
-    ensures forall k | k in Parent().Model().Keys-Traversed() :: key(Peek()) <= k
-  { peekProperties();
-    (stack[0].key,stack[0].value) }
-  
-  lemma {:verify false} peekProperties()
-  requires Valid() 
-  requires stack!=[]
-  requires 0<=|Traversed()|< |Parent().Model().Keys|;
-  ensures (stack[0].key,stack[0].value) in  Parent().Model().Items
-  ensures stack[0].key==elemth(Parent().Model().Keys,|Traversed()|)  
-  ensures stack[0].key !in Traversed()
-  ensures stack[0].value == Parent().Model()[stack[0].key]
-  ensures forall k | k in Traversed() :: k < stack[0].key
-  ensures forall k | k in Parent().Model().Keys-Traversed() :: stack[0].key <= k
-  ensures forall k | k in Parent().Model().Keys-Traversed()-{stack[0].key} :: stack[0].key < k
-  { assert Tree.ValidRec(stack[0],stackSK[0]);
-    assert Tree.SearchTreeRec(stackSK[0]);
-    assert stack[0] in elems(stackSK[0]);
-    Tree.ModelRelationWithSkeletonRecL(stack[0],stackSK[0],stack[0].key,stack[0].value);
-    assert (stack[0].key,stack[0].value) in Tree.MapModelRec(stackSK[0]).Items;
-    parent.tree.mapModelRecContained(stack[0],stackSK[0],parent.tree.root,parent.tree.skeleton);
-    assert Tree.MapModelRec(stackSK[0]).Items <= Parent().Model().Items;
-    assert forall k | k in Parent().Model().Keys-Traversed() && k!=stack[0].key :: stack[0].key < k;
-    lelemthrev(Parent().Model().Keys, stack[0].key, |Traversed()|);
-
-  }
-
- function method HasNext(): bool
-    reads this, Parent(), Parent().Repr()
-    requires Valid()
-    requires Parent().Valid()
-    ensures HasNext()  <==> Traversed() < Parent().Model().Keys && |Traversed()| < |Parent().Model().Keys|
-    //|Traversed()| < |Parent().Model()| es necesario para poder verificar con cota |s.Model()|-|it.Traversed()|
-    ensures !HasNext() ==> Traversed() == Parent().Model().Keys && |Traversed()| == |Parent().Model().Keys|
-  { hasNextProperties();
-    stack != []
-  }
-
-lemma {:verify false} hasNextProperties()
-  requires Valid() 
-  ensures stack!=[] ==> Traversed() < Parent().Model().Keys && |Traversed()| < |Parent().Model().Keys|
-  ensures stack==[] ==> Traversed() == Parent().Model().Keys && |Traversed()| == |Parent().Model().Keys|
-{ if (stack!=[])
-   {
-   //assert stack[0].key in Parent().Model().Keys && stack[0].key !in Traversed();
-   sizesStrictContained(Traversed(),Parent().Model().Keys);
-   }
-
-}
-
-
-  function method Index(): int
-    reads this, Parent(), Parent().Repr()
-    requires Valid()
-    requires Parent().Valid()
-    ensures HasNext() ==> Index()==|Traversed()|==|smaller(Parent().Model().Keys,key(Peek()))|
-    ensures !HasNext() ==> Index()==|Parent().Model()|
-   { traversedRelation();
-     index }
-
-  method Next() returns (p: pairKV)
-    modifies this
-    requires Valid()
-    requires Parent().Valid()
-    requires HasNext()
-    requires allocated(Parent())
-    requires forall it | it in Parent().Repr() :: allocated(it)
-    ensures Parent().Valid()
-    ensures Valid()
-    ensures old(Parent()) == Parent()
-    ensures old(Parent().Model()) == Parent().Model()
-
-    ensures forall x {:trigger x in Parent().Repr(), x in old(Parent().Repr())} | x in Parent().Repr() - old(Parent().Repr()) :: fresh(x)
-    ensures fresh(Parent().Repr()-old(Parent().Repr()))
-    ensures forall x | x in Parent().Repr() :: allocated(x)
-
-    ensures Parent().Iterators() == old(Parent().Iterators())
-
-    ensures p==old(Peek()) && Traversed() == {old(key(Peek()))}+old(Traversed())
-    ensures |Traversed()|==1+|old(Traversed())|
-    ensures HasNext() ==> key(Peek())==elemth(Parent().Model().Keys,|Traversed()|)//already known
-
-    ensures forall it | it in Parent().Iterators() && old(it.Valid()) ::
-      it.Valid() && (it != this ==> it.Traversed() == old(it.Traversed()) && (it.HasNext() ==> it.Peek()==old(it.Peek())))
-
-function method HasPrev(): bool//igual que HasNext
-    reads this, Parent(), Parent().Repr()
-    requires Valid()
-    requires Parent().Valid()
-    ensures HasPrev()  <==> Traversed() < Parent().Model().Keys && |Traversed()| < |Parent().Model().Keys|
-    //|Traversed()| < |Parent().Model()| es necesario para poder verificar con cota |s.Model()|-|it.Traversed()|
-    ensures !HasPrev() ==> Traversed() == Parent().Model().Keys && |Traversed()| == |Parent().Model().Keys|
-  {hasNextProperties();
-   stack!=[]
-  }
-
-  method Prev() returns (p: pairKV)
-    modifies this
-    requires Valid()
-    requires Parent().Valid()
-    requires HasNext() 
-    requires allocated(Parent())
-    requires forall it | it in Parent().Repr() :: allocated(it)
-    ensures Parent().Valid()
-    ensures Valid()
-    ensures old(Parent()) == Parent()
-    ensures old(Parent().Model()) == Parent().Model()
-
-    ensures forall x {:trigger x in Parent().Repr(), x in old(Parent().Repr())} | x in Parent().Repr() - old(Parent().Repr()) :: fresh(x)
-    ensures fresh(Parent().Repr()-old(Parent().Repr()))
-    ensures forall x | x in Parent().Repr() :: allocated(x)
-
-    ensures Parent().Iterators() == old(Parent().Iterators())
-    ensures p==old(Peek())  
-    ensures old(Traversed())=={} ==> Traversed()==Parent().Model().Keys
-    ensures old(Traversed())!={} ==> (Traversed()==old(Traversed())-{maximum(old(Traversed()))} &&
-                                      (HasNext() ==> key(Peek())==maximum(old(Traversed()))))
-    ensures forall it | it in Parent().Iterators() && old(it.Valid()) ::
-      it.Valid() && (it != this ==> it.Traversed() == old(it.Traversed()) && (it.HasNext() ==> it.Peek()==old(it.Peek())))
-
-  method Copy() returns (it: UnorderedMapIterator)
-    modifies Parent(), Parent().Repr()
-    requires Valid()
-    requires Parent().Valid()
-    requires allocated(Parent())
-    requires forall it | it in Parent().Iterators() :: allocated(it)
-    ensures fresh(it)
-    ensures Valid()
-    ensures Parent() == old(Parent())
-    ensures Parent().Valid()
-    ensures Parent().Model() == old(Parent().Model())
-
-    ensures forall x {:trigger x in Parent().Repr(), x in old(Parent().Repr())} | x in Parent().Repr() - old(Parent().Repr()) :: fresh(x)
-    ensures fresh(Parent().Repr()-old(Parent().Repr()))
-    ensures forall x | x in Parent().Repr() :: allocated(x)
-    
-    ensures it is OrderedMapIterator
-    ensures it.Valid()
-    ensures Parent().Iterators() == {it} + old(Parent().Iterators())
-    ensures Parent() == it.Parent()
-
-    ensures Traversed() == it.Traversed() 
-    ensures HasNext() ==> Peek()==it.Peek()
-    ensures forall it | it in old(Parent().Iterators()) && old(it.Valid()) ::
-      it.Valid() && it.Traversed() == old(it.Traversed()) && (it.HasNext() ==> it.Peek()==old(it.Peek()))
-
-}
-
 class OrderedMapImpl extends OrderedMap {
-  
- var  tree:Tree;
-  ghost var iters:set<OrderedMapIteratorImpl>;
-
-
-  constructor()
-  ensures Valid()
-  ensures Model()==map[]
-  ensures fresh(Repr())
-  ensures forall x | x in Repr() :: fresh(x) 
-  {
-   tree:=new Tree();
-   iters:={};
-
-  }
+  var tree: SearchTree;
+  //ghost var iters: set<OrderedMapIteratorImpl>;
 
   function Repr0(): set<object>
     reads this
   {
-    {tree} + iters 
+    {tree} // + iters
   }
 
-function Repr1(): set<object>
+  function Repr1(): set<object>
     reads this, Repr0()
   {
-    Repr0() + tree.Repr()
+    Repr0() + {tree.tree}
   }
+
+  function Repr2(): set<object>
+    reads this, Repr1()
+  {
+    Repr1() + tree.tree.Repr()
+  }
+
   function ReprDepth(): nat
     reads this
     ensures ReprDepth() > 0
-  { 1 }
+  { 2 }
 
   function ReprFamily(n: nat): set<object>
     decreases n
@@ -719,10 +35,10 @@ function Repr1(): set<object>
     ensures n > 0 ==> ReprFamily(n) >= ReprFamily(n-1)
     reads this, if n == 0 then {} else ReprFamily(n-1)
   {
-    if (n==0) then Repr0()
-    else Repr1()
+    if n == 0 then Repr0()
+    else if n == 1 then Repr1()
+    else Repr2()
   }
-  
 
   lemma UselessLemma()
     ensures Repr() == ReprFamily(ReprDepth());
@@ -730,33 +46,47 @@ function Repr1(): set<object>
   predicate Valid()
     reads this, Repr()
   {
-   tree.Valid() && tree.SearchTree()&&
-   forall it | it in iters :: it.parent==this && {it}!!{this}
-  }  
+    tree.Valid()
+    //&& (forall it | it in iters :: it.parent == this && {it} !! {this})
+  }
 
   function Model(): map<K,V>
     reads this, Repr()
     requires Valid()
   {
-    tree.MapModel()
+    tree.tree.Model()
   }
 
-function method Empty(): bool
+  constructor()
+    ensures Valid()
+    ensures Model() == map[]
+    ensures forall x {:trigger x in Repr(), x in old(Repr())} | x in Repr() :: fresh(x)
+    ensures fresh(Repr())
+    ensures forall x | x in Repr() :: allocated(x)
+  {
+    tree := new SearchTree();
+    new;
+    assert Repr() == {tree} + {tree.tree} + tree.tree.Repr();
+    assert fresh(tree.Repr());
+    assert tree.Repr() == tree.tree.Repr();
+    assert fresh(tree.tree.Repr());
+    assert fresh(Repr());
+  }
+
+  function method Empty(): bool
     reads this, Repr()
     requires Valid()
     ensures Empty() <==> Model() == map[]
-  { 
-    tree.isEmpty() 
+  {
+    tree.tree.isEmpty()
   }
-
-
 
  function method Size(): nat
     reads this, Repr()
     requires Valid()
     ensures Size() == |Model()|
-  { 
-    tree.Size() 
+  {
+    tree.tree.Size()
   }
 
  function Iterators(): set<UnorderedMapIterator>
@@ -764,9 +94,11 @@ function method Empty(): bool
     requires Valid()
     ensures forall it | it in Iterators() :: it in Repr() && it.Parent() == this
     ensures forall it | it in Iterators() :: it is OrderedMapIterator
-  { iters }
+  {
+    {} //iters
+  }
 
-method First() returns (it: UnorderedMapIterator)
+  method First() returns (it: UnorderedMapIterator)
     modifies this, Repr()
     requires Valid()
     requires forall x | x in Repr() :: allocated(x)
@@ -783,17 +115,19 @@ method First() returns (it: UnorderedMapIterator)
     ensures fresh(it)
     ensures it.Valid()
     ensures it.Parent() == this
-    ensures it.Traversed()=={} 
+    ensures it.Traversed()=={}
     ensures Model()!=map[] ==> it.HasNext() && key(it.Peek())==elemth(Model().Keys,0)
     ensures Iterators() == {it} + old(Iterators())
     ensures forall it | it in old(Iterators()) && old(it.Valid()) ::
       it.Valid() && it.Traversed() == old(it.Traversed()) && (it.HasNext() ==> it.Peek()==old(it.Peek()))
-    {
-     var  iter:=new OrderedMapIteratorImpl(this);
-       iters:=iters+{iter};
-      it :=iter;
-      assume false;
-     }
+  /*
+  {
+    var  iter := new OrderedMapIteratorImpl(this);
+    iters := iters+{iter};
+    it := iter;
+    assume false;
+  }
+  */
 
 
   method Last() returns (it: OrderedMapIterator)//iterator to the last element
@@ -816,63 +150,60 @@ method First() returns (it: UnorderedMapIterator)
     ensures forall it | it in old(Iterators()) && old(it.Valid()) ::
       it.Valid() && it.Traversed() == old(it.Traversed()) && (it.HasNext() ==> it.Peek()==old(it.Peek()))
 
-method contains(k:K) returns (b:bool)
+  method contains(k:K) returns (b:bool)
     requires Valid()
     requires forall x | x in Repr() :: allocated(x)
-    
-    ensures Valid() 
-    ensures b==(k in Model()) 
+
+    ensures Valid()
+    ensures b==(k in Model())
 
     ensures forall x {:trigger x in Repr(), x in old(Repr())} | x in Repr() - old(Repr()) :: fresh(x)
     ensures fresh(Repr()-old(Repr()))
     ensures forall x | x in Repr() :: allocated(x)
-   
+
     ensures Iterators() == old(Iterators())
   {
-   assert tree.Repr() <= Repr();
-
-   b:=tree.Search(k);
-
+    assert tree.tree.Repr() <= Repr();
+    b := tree.Search(k);
   }
 
-method at(k:K) returns (v:V)
+  method at(k:K) returns (v:V)
     //modifies this,Repr()
     requires Valid()
     requires forall x | x in Repr() :: allocated(x)
     requires k in Model()
     ensures Valid()
     //ensures Model()==old(Model())
-    ensures v == Model()[k] 
+    ensures v == Model()[k]
 
     ensures forall x {:trigger x in Repr(), x in old(Repr())} | x in Repr() - old(Repr()) :: fresh(x)
     ensures fresh(Repr()-old(Repr()))
     ensures forall x | x in Repr() :: allocated(x)
-   
+
     ensures Iterators() == old(Iterators())
   {
-    assert tree.Repr() <= Repr();
-
-    v:=tree.Get(k);
+    assert tree.tree.Repr() <= Repr();
+    v := tree.Get(k);
   }
 
 
- method add(k:K,v:V)
-    modifies this,Repr()
+  method add(k: K, v: V)
+    modifies this, Repr()
     requires Valid()
-    requires forall x | x in Repr() :: allocated(x)
     ensures Valid()
-    ensures Model() == old(Model())[k:=v] 
+    ensures Model() == old(Model())[k := v]
 
+    requires forall x | x in Repr() :: allocated(x)
     ensures forall x {:trigger x in Repr(), x in old(Repr())} | x in Repr() - old(Repr()) :: fresh(x)
     ensures fresh(Repr()-old(Repr()))
     ensures forall x | x in Repr() :: allocated(x)
-   
+
     ensures Iterators() == old(Iterators())
   {
-    tree.Insert(k,v);
+    tree.Insert(k, v);
   }
 
-method remove(k:int) 
+  method remove(k:int)
     modifies this,Repr()
     requires Valid()
     requires forall x | x in Repr() :: allocated(x)
@@ -885,21 +216,18 @@ method remove(k:int)
 
     ensures Iterators() == old(Iterators())
   {
-   tree.Remove(k);
+    tree.Remove(k);
   }
 
-
-
-
-method find(k:K) returns (newt:UnorderedMapIterator)
+  method find(k:K) returns (newt:UnorderedMapIterator)
     modifies this, Repr()
     requires Valid()
     requires forall x | x in Repr() :: allocated(x)
-    ensures Valid() 
+    ensures Valid()
     ensures Model()==old(Model())
-    
+
     ensures newt is OrderedMapIterator
-    ensures fresh(newt) 
+    ensures fresh(newt)
     ensures newt.Valid() && newt.Parent()==this
     ensures k in old(Model()) ==> newt.HasNext() && key(newt.Peek())==k
     ensures k !in old(Model()) ==> newt.Traversed()==Model().Keys
@@ -913,17 +241,17 @@ method find(k:K) returns (newt:UnorderedMapIterator)
   method insert(mid: UnorderedMapIterator, k: K, v : V) returns (newt:UnorderedMapIterator)
     modifies this, Repr()
     requires Valid()
-    requires mid.Valid() 
+    requires mid.Valid()
     requires mid.Parent() == this
     requires mid in Iterators()
     requires forall x | x in Repr() :: allocated(x)
     ensures Valid()
-    ensures Model() == old(Model())[k:=v]
+    ensures Model() == old(Model())[k := v]
 
     ensures newt is OrderedMapIterator
     ensures fresh(newt)
     ensures Iterators() == {newt}+old(Iterators())
-    ensures newt.Valid() && newt.Parent()==this  
+    ensures newt.Valid() && newt.Parent()==this
     ensures newt.HasNext() && newt.Peek()==(k,v) && newt.Traversed()==smaller(Model().Keys,k)
 
     ensures forall x {:trigger x in Repr(), x in old(Repr())} | x in Repr() - old(Repr()) :: fresh(x)
@@ -931,7 +259,7 @@ method find(k:K) returns (newt:UnorderedMapIterator)
     ensures forall x | x in Repr() :: allocated(x)
 
     //points either to the inserted elemento or to the already existing one
- 
+
 
 
 
@@ -945,11 +273,11 @@ method find(k:K) returns (newt:UnorderedMapIterator)
     requires forall x | x in Repr() :: allocated(x)
     ensures Valid()
     ensures Model()== map k | k in old(Model()) && k!=old(key(mid.Peek()))::old(Model())[k]
-    
+
     ensures next is OrderedMapIterator
     ensures fresh(next)
     ensures Iterators() == {next}+old(Iterators())
-    ensures next.Valid() && next.Parent()==this 
+    ensures next.Valid() && next.Parent()==this
     ensures next.Traversed()==old(mid.Traversed()) &&
                 (next.HasNext() ==> key(next.Peek())==elemth(Model().Keys,|next.Traversed()|) && value(next.Peek())==Model()[key(next.Peek())])
 
@@ -957,5 +285,4 @@ method find(k:K) returns (newt:UnorderedMapIterator)
     ensures forall x {:trigger x in Repr(), x in old(Repr())} | x in Repr() - old(Repr()) :: fresh(x)
     ensures fresh(Repr()-old(Repr()))
     ensures forall x | x in Repr() :: allocated(x)
- 
 }
